{-# OPTIONS --prop --rewriting #-}

module ZF where
open import Agda.Builtin.Equality
open import Agda.Primitive
open import logic
open _âˆ§_

postulate
    -- We postulate a universe of sets, and a _âˆˆ_ relation between them.
    ğ• : Set
    _âˆˆ_ : ğ• -> ğ• -> Prop
{-# INJECTIVE _âˆˆ_ #-}
infix 20 _âˆˆ_

private variable
    â„“ â„“â‚ â„“â‚‚ â„“â‚ƒ â„“â‚„ â„“â‚… â„“â‚† â„“â‚‡ â„“â‚ˆ â„“' â„“'' : Level
    x y z w : ğ•  -- These will range over sets unless noted otherwise.

-- A propositional equality for convenience.
-- We avoid the use of this as much as possible.
data _â‰—_ : ğ• -> ğ• -> Prop where
    reflğ• : x â‰— x

-- The _âˆˆ_ relation is extensional. The elements of (_âˆˆ x) uniquely defines x.
postulate
    Extensional : (âˆ€ z -> z âˆˆ x â‰¡ z âˆˆ y) -> x â‰¡ y
-- The converse holds by Leibniz's law.
Extensional-converse : x â‰¡ y -> (âˆ€ z -> z âˆˆ x â‰¡ z âˆˆ y)
Extensional-converse refl z = refl

-- Extensionality flattens the propositional equality into the regular one.
â‰—-â‰¡ : x â‰— y -> x â‰¡ y
â‰—-â‰¡ eq = Extensional (\ z -> equiv-equal (ex eq z))
    where
        ex : x â‰— y -> (z : ğ•) -> (z âˆˆ x -> z âˆˆ y) âˆ§ (z âˆˆ y -> z âˆˆ x)
        ex reflğ• z = [ idP , idP ]

â‰¡-â‰— : x â‰¡ y -> x â‰— y
â‰¡-â‰— refl = reflğ•

_â‰Ÿ_ : {A : Set â„“} (x y : ğ•) -> (x â‰¡ y) âŠ (x â‰¡ y -> A)
x â‰Ÿ y with truth (x â‰— y)
... | injâ‚ eq = injâ‚ (â‰—-â‰¡ (â‰¡-true eq))
... | injâ‚‚ neq = injâ‚‚ \ { refl -> magic (â‰¡-false neq reflğ•) }

-- We postulate the existence of an empty set, i.e. a set with no elements
-- This is actually redundant from the other axioms, but we keep it for
-- aesthetic considerations.
postulate
    âˆ… : ğ•
    âˆ…-empty : x âˆˆ âˆ… â‰¡ âŠ¥

{-# REWRITE âˆ…-empty #-}

-- From extensionality, we immediately obtain that the empty set is unique.
âˆ…-unique : (âˆ€ x -> x âˆˆ y â‰¡ âŠ¥) -> y â‰¡ âˆ…
âˆ…-unique = Extensional  -- Well, that's literally immediate.

-- Conversely, every non-empty set has an element.
-- This crucially depends on the principle of excluded middle.
non-empty : (x â‰¢ âˆ…) -> âˆƒ[ y âˆˆ ğ• ] (y âˆˆ x)
non-empty {x} neq with Îµ[ y âˆˆ ğ• ] (y âˆˆ x)
... | Î¹â‚ no =            -- Case 1 : y contains no element,
        neq                  -- y is not the empty set (assumption), but
        (âˆ…-unique \ y ->     -- y is the empty set, since
            false-â‰¡ (no y))  -- y is contains no element. (assumption)
    ThusFrom ex-falso        -- Contradiction!
... | Î¹â‚‚ yes = yes       -- Case 2 : y contains an element, QED.

-- We define the subset relation.
_âŠ†_ : ğ• -> ğ• -> Prop
x âŠ† y = âˆ€ {z} -> z âˆˆ x -> z âˆˆ y

xâŠ†âˆ…-â‰¡ : x âŠ† âˆ… -> x â‰¡ âˆ…
xâŠ†âˆ…-â‰¡ s = âˆ…-unique \ y -> false-â‰¡ s

xâŠ†âˆ… : (x âŠ† âˆ…) â‰¡ (x â‰— âˆ…)
xâŠ†âˆ… = equiv-equal [ (\ xâŠ†âˆ… -> â‰¡-â‰— (xâŠ†âˆ…-â‰¡ xâŠ†âˆ…)) , (\{ reflğ• -> idP }) ]

-- We postulate the existence of power sets.
postulate
    ğ’« : ğ• -> ğ•
    Power : (x : ğ•)
        -> âˆ€ z -> z âˆˆ ğ’« x â‰¡ z âŠ† x
{-# REWRITE Power #-}

-- The empty set is in every power set.
âˆ…âˆˆğ’«x : âˆ… âˆˆ ğ’« x
âˆ…âˆˆğ’«x ()

-- The whole set is in every power set.
xâˆˆğ’«x : x âˆˆ ğ’« x
xâˆˆğ’«x i = i

ğŸ™ : ğ•  -- the singleton set
ğŸ™ = ğ’« âˆ…

ğŸ™-singleton : (x âˆˆ ğŸ™) -> (x â‰¡ âˆ…)
ğŸ™-singleton s = Extensional \ z -> false-â‰¡ s

-- ğŸ™ is not âˆ…
âˆ…â‰¢ğŸ™ : âˆ… â‰¢ ğŸ™
âˆ…â‰¢ğŸ™ eq = equal-equiv {P = âˆ… âˆˆ ğŸ™} {Q = âˆ… âˆˆ âˆ…} Pâ‰¡Q (xâˆˆğ’«x {x = âˆ…} {z = âˆ…})
    where
        Pâ‰¡Q : âˆ… âˆˆ ğŸ™ â‰¡ âˆ… âˆˆ âˆ…
        Pâ‰¡Q = cong (\ z -> âˆ… âˆˆ z) (symm eq)

ğŸš : ğ•  -- The boolean set
ğŸš = ğ’« ğŸ™

ğŸš-boolean : (x âˆˆ ğŸš) -> (x â‰¡ âˆ…) âŠ (x â‰¡ ğŸ™)
ğŸš-boolean {x = x} xâˆˆğŸš
    -- We see if x is empty.
    with truth {lzero} (âˆ€ y -> (y âˆˆ x) -> âŠ¥)
... | injâ‚ is-empty = injâ‚ (âˆ…-unique  -- x has no elements, then by extensionality
                                      -- we just need to prove that x is empty.
    \ y -> false-â‰¡                    -- If y is in x,
    \ yâˆˆx -> â‰¡-true is-empty y yâˆˆx )  -- By definition, we get contradiction.
... | injâ‚‚ non-empty = injâ‚‚ (Extensional  -- x is non-empty, we invoke extensionality.
    \ z -> equiv-equal
        [ xâˆˆğŸš , zâˆˆx z ])
    where
        zâˆˆx : âˆ€ z -> z âŠ† âˆ… -> z âˆˆ x
        zâˆˆx z zâŠ†âˆ… rewrite xâŠ†âˆ…-â‰¡ {z} zâŠ†âˆ…
            with choice-safe (â‰¡-false non-empty)
        ... | exists a aâˆˆx rewrite symm (âˆ…-unique {y = a} (\ z -> false-â‰¡ (xâˆˆğŸš aâˆˆx)))
            = aâˆˆx

postulate
    â‹ƒ : ğ• -> ğ•
    Union : (x : ğ•) -> z âˆˆ â‹ƒ x â‰¡ âˆƒ[ y âˆˆ ğ• ] (z âˆˆ y âˆ§ y âˆˆ x)
{-# REWRITE Union #-}

-- Union and powerset are "sort of" inverse to each other.
-- â‹ƒ (ğ’« x) = x, but ğ’« (â‹ƒ x) âŠ‡ x.
â‹ƒ-ğ’« : â‹ƒ (ğ’« x) â‰¡ x
â‹ƒ-ğ’« {x = x} = Extensional
    \ z -> equiv-equal
        [ zig , zag ]
    where
        zig : z âˆˆ â‹ƒ (ğ’« x) -> z âˆˆ x
        zig (exists a [ zâˆˆa , aâŠ†x ]) = aâŠ†x zâˆˆa
        zag : z âˆˆ x -> z âˆˆ â‹ƒ (ğ’« x)
        zag i = exists x [ i , idP ]

ğ’«-â‹ƒ : x âŠ† ğ’« (â‹ƒ x)
ğ’«-â‹ƒ zâˆˆx yâˆˆz = exists _ [ yâˆˆz , zâˆˆx ]

â‹ƒâˆ…â‰¡âˆ… : â‹ƒ âˆ… â‰¡ âˆ…
â‹ƒâˆ…â‰¡âˆ… = Extensional
    \ _ -> false-â‰¡
    \ { (exists _ ()) }

-- These two are direct application of the almost-inverse relation.
â‹ƒğŸ™â‰¡âˆ… : â‹ƒ ğŸ™ â‰¡ âˆ…
â‹ƒğŸ™â‰¡âˆ… = â‹ƒ-ğ’«
â‹ƒğŸšâ‰¡ğŸ™ : â‹ƒ ğŸš â‰¡ ğŸ™
â‹ƒğŸšâ‰¡ğŸ™ = â‹ƒ-ğ’«

-- Since Agda wants the syntax { } and â¦ƒ â¦„ very much, we will avoid this.
-- Instead, we use âŸ¦ âŸ§ as set builders.
postulate
    Comprehension : (x : ğ•) -> (P : ğ• -> Prop) -> ğ•
    Specification : (P : ğ• -> Prop)
        -> z âˆˆ Comprehension x P â‰¡ (z âˆˆ x âˆ§ P z)
{-# REWRITE Specification #-}
syntax Comprehension x (\ y -> P) = âŸ¦ y âˆˆ x âˆ¥ P âŸ§
infix 6 Comprehension

module Intersection where
    abstract
        -- Now intersections can be defined.
        â‹‚ : ğ• -> ğ•
        â‹‚ x = âŸ¦ y âˆˆ â‹ƒ x âˆ¥ (âˆ€ w -> w âˆˆ x -> y âˆˆ w) âŸ§
        -- We can't prove much interesting stuff about intersections yet.

        Intersection-definition : â‹‚ x â‰¡ âŸ¦ y âˆˆ â‹ƒ x âˆ¥ (âˆ€ w -> w âˆˆ x -> y âˆˆ w) âŸ§
        Intersection-definition = refl

        Intersection : (x y : ğ•) -> y âˆˆ â‹‚ x â‰¡
            (âˆƒ[ z âˆˆ ğ• ] (y âˆˆ z âˆ§ z âˆˆ x)) âˆ§ (âˆ€ w -> w âˆˆ x -> y âˆˆ w)
        Intersection x y = refl
open Intersection public
{-# REWRITE Intersection #-}

module Singleton where
    abstract
        -- We can also define singleton sets now.
        âŸ¦_âŸ§ : ğ• -> ğ•
        âŸ¦ x âŸ§ = âŸ¦ w âˆˆ ğ’« x âˆ¥ w â‰— x âŸ§

        -- Singletons are really singletons.
        âŸ¦_âŸ§-singleton : (x : ğ•) {y : ğ•} -> y âˆˆ âŸ¦ x âŸ§ -> y â‰¡ x
        âŸ¦ x âŸ§-singleton [ yâŠ†x , yâ‰—x ] = â‰—-â‰¡ yâ‰—x

        Singleton : (y âˆˆ âŸ¦ x âŸ§) â‰¡ (y â‰— x)
        Singleton = equiv-equal [ Ï€â‚‚ , (\ { reflğ• -> [ idP , reflğ• ]}) ]
open Singleton public
{-# REWRITE Singleton #-}

-- ğŸ™ is equivalently defined as a singleton.
ğŸ™â‰¡âŸ¦âˆ…âŸ§ : ğŸ™ â‰¡ âŸ¦ âˆ… âŸ§
ğŸ™â‰¡âŸ¦âˆ…âŸ§ = Extensional
    \ z -> equiv-equal
    [ (\ u -> â‰¡-â‰— (xâŠ†âˆ…-â‰¡ u)) , (\ { reflğ• -> idP }) ]

-- To unwrap a singleton, take the union.
â‹ƒâŸ¦xâŸ§ : â‹ƒ âŸ¦ x âŸ§ â‰¡ x
â‹ƒâŸ¦xâŸ§ = Extensional
    \ z -> equiv-equal
    [ (\ { (exists _ [ zâˆˆx , reflğ• ]) -> zâˆˆx }) , (\ zâˆˆx -> exists _ [ zâˆˆx , reflğ• ]) ]

postulate
    Image : (x : ğ•) {_â†¦_ : ğ• -> ğ• -> Prop} -> (âˆ€ y -> y âˆˆ x -> âˆƒ![ z âˆˆ ğ• ] y â†¦ z) -> ğ•
    Replacement : (x : ğ•) {_â†¦_ : ğ• -> ğ• -> Prop}
        -> (unique : âˆ€ y -> y âˆˆ x -> âˆƒ![ z âˆˆ ğ• ] y â†¦ z)
        -> (âˆ€ z -> z âˆˆ Image x unique â‰¡ âˆƒ[ y âˆˆ ğ• ] (y âˆˆ x âˆ§ y â†¦ z))
{-# REWRITE Replacement #-}

-- Now we can *really* start to make sets.
-- For a start, we prove Pairing, i.e. {a, b} is a set
-- We first need to get a predicate to replace.
private  -- Start a private block since we don't want to contaminate the namespace
    Pair : ğ• -> ğ• -> ğ• -> ğ• -> Prop
    Pair a b x y = (x â‰— âˆ… âˆ§ y â‰— a) âˆ¨ (x â‰— ğŸ™ âˆ§ y â‰— b)
    -- Now let's prove that it is indeed a map!
    Pair-unique : âˆ€ a b -> âˆ€ y -> y âˆˆ ğŸš -> âˆƒ![ z âˆˆ ğ• ] (Pair a b y z)
    Pair-unique a b y yâˆˆğŸš with ğŸš-boolean {x = y} yâˆˆğŸš
    ... | injâ‚ refl = exists-unique a \ w ->
        \ { pairing -> â‰—-â‰¡ (wâ‰—a w pairing) }
        where
            wâ‰—a : âˆ€ w -> (âˆ… â‰— âˆ…) âˆ§ (w â‰— a) âˆ¨ (âˆ… â‰— ğŸ™) âˆ§ (w â‰— b) -> w â‰— a
            wâ‰—a w (Î¹â‚ left) = Ï€â‚‚ left
            wâ‰—a w (Î¹â‚‚ [ âˆ…â‰—ğŸ™ , _ ]) = ex-falso (âˆ…â‰¢ğŸ™ (â‰—-â‰¡ âˆ…â‰—ğŸ™))
    ... | injâ‚‚ refl = exists-unique b \ w ->
        \ { pairing -> â‰—-â‰¡ (wâ‰—b w pairing) }
        where
            wâ‰—b : âˆ€ w -> (ğŸ™ â‰— âˆ…) âˆ§ (w â‰— a) âˆ¨ (ğŸ™ â‰— ğŸ™) âˆ§ (w â‰— b) -> w â‰— b
            wâ‰—b w (Î¹â‚‚ right) = Ï€â‚‚ right
            wâ‰—b w (Î¹â‚ [ ğŸ™â‰—âˆ… , _ ]) = ex-falso (âˆ…â‰¢ğŸ™ (symm (â‰—-â‰¡ ğŸ™â‰—âˆ…)))

module Pairing where
    abstract
        âŸ¨_,_âŸ© : ğ• -> ğ• -> ğ•
        âŸ¨ x , y âŸ© = Image ğŸš (Pair-unique x y)
        Pair-definition : âŸ¨ x , y âŸ© â‰¡ Image ğŸš (Pair-unique x y)
        Pair-definition = refl

        private
            Pairing-> : z âˆˆ âŸ¨ x , y âŸ© -> (z â‰— x) âˆ¨ (z â‰— y)
            Pairing-> (exists a [ aâˆˆğŸš , pairing ]) with ğŸš-boolean {x = a} aâˆˆğŸš
            Pairing-> (exists âˆ… [ aâˆˆğŸš , Î¹â‚ [ _ , zâ‰—x ] ]) | injâ‚ refl = Î¹â‚ zâ‰—x
            Pairing-> (exists âˆ… [ aâˆˆğŸš , Î¹â‚‚ [ âˆ…â‰—ğŸ™ , _ ] ]) | injâ‚ refl = ex-falso (âˆ…â‰¢ğŸ™ (â‰—-â‰¡ âˆ…â‰—ğŸ™))
            Pairing-> (exists ğŸ™ [ aâˆˆğŸš , Î¹â‚ [ ğŸ™â‰—âˆ… , _ ] ]) | injâ‚‚ refl = ex-falso (âˆ…â‰¢ğŸ™ (symm (â‰—-â‰¡ ğŸ™â‰—âˆ…)))
            Pairing-> (exists ğŸ™ [ aâˆˆğŸš , Î¹â‚‚ [ _ , zâ‰—y ] ]) | injâ‚‚ refl = Î¹â‚‚ zâ‰—y

            Pairing<- : (z â‰— x) âˆ¨ (z â‰— y) -> z âˆˆ âŸ¨ x , y âŸ©
            Pairing<- (Î¹â‚ reflğ•)
                = exists âˆ… [ ex-falso , Î¹â‚ [ reflğ• , reflğ• ] ]
            Pairing<- (Î¹â‚‚ reflğ•)
                = exists ğŸ™ [ idP , Î¹â‚‚ [ reflğ• , reflğ• ] ]
        
        Pairing : z âˆˆ âŸ¨ x , y âŸ© â‰¡ (z â‰— x) âˆ¨ (z â‰— y)
        Pairing = equiv-equal [ Pairing-> , Pairing<- ]
open Pairing public

{-# REWRITE Pairing #-}

Pairing-â‰¡ : z âˆˆ âŸ¨ x , y âŸ© -> (z â‰¡ x) âŠ (z â‰¡ y)
Pairing-â‰¡ {z = z} {x = x} {y = y} i with âˆ¨-oracle (true-â‰¡ i)
... | injâ‚ l = injâ‚ (â‰—-â‰¡ (â‰¡-true l))
... | injâ‚‚ r = injâ‚‚ (â‰—-â‰¡ (â‰¡-true r))

-- For example, ğŸš is equal to âŸ¨ âˆ… , ğŸ™ âŸ©.
ğŸšâ‰¡âŸ¨âˆ…,ğŸ™âŸ© : ğŸš â‰¡ âŸ¨ âˆ… , ğŸ™ âŸ©
ğŸšâ‰¡âŸ¨âˆ…,ğŸ™âŸ© = Extensional \ z ->
    equiv-equal [ zig z , zag z ]
    where
        zig : âˆ€ z -> z âˆˆ ğŸš -> z âˆˆ âŸ¨ âˆ… , ğŸ™ âŸ©
        zig z i with ğŸš-boolean {x = z} i
        ... | injâ‚ refl = Î¹â‚ reflğ•
        ... | injâ‚‚ refl = Î¹â‚‚ reflğ•
        zag : âˆ€ z -> z âˆˆ âŸ¨ âˆ… , ğŸ™ âŸ© -> z âˆˆ ğŸš
        zag .âˆ… (Î¹â‚ reflğ•) ()
        zag .(ğ’« âˆ…) (Î¹â‚‚ reflğ•) i = i

-- Pairs are unordered.
Pair-unordered : âˆ€ x y -> âŸ¨ x , y âŸ© â‰¡ âŸ¨ y , x âŸ©
Pair-unordered x y = Extensional \ z ->
    equiv-equal [ zig x y z , zig y x z ]
    where
        zig : âˆ€ x y z -> z âˆˆ âŸ¨ x , y âŸ© -> z âˆˆ âŸ¨ y , x âŸ©
        zig x y .x (Î¹â‚ reflğ•) = Î¹â‚‚ reflğ•
        zig x y .y (Î¹â‚‚ reflğ•) = Î¹â‚ reflğ•

-- We have a criterion for pair equality.
-- To prove that cleanly, we first develop some tools.
private
    Pair-equal-left : âˆ€ x y z w -> âŸ¨ x , y âŸ© â‰¡ âŸ¨ z , w âŸ© -> (x â‰— z) âˆ¨ (x â‰— w)
    Pair-equal-left x y z w eq 
        = equal-equiv (Extensional-converse eq x) (Î¹â‚ reflğ•)

    Pair-equal-right : âˆ€ x y z w -> âŸ¨ x , y âŸ© â‰¡ âŸ¨ z , w âŸ© -> (y â‰— w) âˆ¨ (y â‰— z)
    Pair-equal-right x y z w eq
        rewrite Pair-unordered x y rewrite Pair-unordered z w
            = Pair-equal-left _ _ _ _ eq

    Pair-equal-equiv : âˆ€ x y z w -> âŸ¨ x , y âŸ© â‰¡ âŸ¨ z , w âŸ©
        -> (x â‰— z) âˆ§ (y â‰— w) âˆ¨ (x â‰— w) âˆ§ (y â‰— z)
    Pair-equal-equiv x y z w eq
        with Pair-equal-left _ _ _ _ eq
        | Pair-equal-right _ _ _ _ eq
    ... | Î¹â‚ xz | Î¹â‚ yw = Î¹â‚ [ xz , yw ]
    ... | Î¹â‚‚ xw | Î¹â‚‚ yz = Î¹â‚‚ [ xw , yz ]
    ... | Î¹â‚ reflğ• | Î¹â‚‚ reflğ• = Î¹â‚ [ reflğ• , xw ]
        where
            xw : x â‰— w
            xw with Pâˆ¨P _
                (equal-equiv
                    (symm (Extensional-converse eq w))
                        (Î¹â‚‚ reflğ•))
            ... | reflğ• = reflğ•
    ... | Î¹â‚‚ reflğ• | Î¹â‚ reflğ• = Î¹â‚‚ [ reflğ• , yz ]
        where
            yz : y â‰— z
            yz with Pâˆ¨P _
                (equal-equiv
                    (symm (Extensional-converse eq z))
                        (Î¹â‚ reflğ•))
            ... | reflğ• = reflğ•

Pair-equal : âŸ¨ x , y âŸ© â‰¡ âŸ¨ z , w âŸ© -> (x â‰¡ z) * (y â‰¡ w) âŠ (x â‰¡ w) * (y â‰¡ z)
Pair-equal {x} {y} {z} {w} eq with âˆ¨-oracle (true-â‰¡ (Pair-equal-equiv x y z w eq))
... | injâ‚ l = let (ll , lr) = âˆ§-oracle l in injâ‚ (â‰—-â‰¡ (â‰¡-true ll) , â‰—-â‰¡ (â‰¡-true lr))
... | injâ‚‚ r = let (rl , rr) = âˆ§-oracle r in injâ‚‚ (â‰—-â‰¡ (â‰¡-true rl) , â‰—-â‰¡ (â‰¡-true rr))

-- Singletons can be alternatively defined as unordered pairs.
singleton-pair : âŸ¦ x âŸ§ â‰¡ âŸ¨ x , x âŸ©
singleton-pair {x} = Extensional \ z -> equiv-equal
    (solve 1 (\ P -> P <=> P ||| P) (z â‰— x))

module Kuratowski where
    abstract
        -- Then, we can have Kuratowski pairs.
        -- This construction cleverly avoids the need for Regularity.
        âŸª_,_âŸ« : ğ• -> ğ• -> ğ•
        âŸª x , y âŸ« = âŸ¨ âŸ¦ x âŸ§ , âŸ¨ x , y âŸ© âŸ©

        -- We can prove that Kuratowski pairs are indeed ordered.
        -- A lemma first
        private
            Pair-zig : âˆ€ x y z w -> (âŸ¨ x , x âŸ© â‰¡ âŸ¨ z , z âŸ©) * (âŸ¨ x , y âŸ© â‰¡ âŸ¨ z , w âŸ©)
                -> (x â‰¡ z) * (y â‰¡ w)
            Pair-zig x y z w (eqâ‚ , eqâ‚‚) with Pair-equal eqâ‚ | Pair-equal eqâ‚‚
            ... | injâ‚ (refl , refl) | injâ‚ (refl , refl) = refl , refl
            ... | injâ‚ (refl , refl) | injâ‚‚ (refl , refl) = refl , refl
            ... | injâ‚‚ (refl , refl) | injâ‚ (refl , refl) = refl , refl
            ... | injâ‚‚ (refl , refl) | injâ‚‚ (refl , refl) = refl , refl

            Pair-zag : âˆ€ x y z w -> (âŸ¨ x , x âŸ© â‰¡ âŸ¨ z , w âŸ©) * (âŸ¨ x , y âŸ© â‰¡ âŸ¨ z , z âŸ©)
                -> (x â‰¡ z) * (y â‰¡ w)
            Pair-zag x y z w (eqâ‚ , eqâ‚‚) with Pair-equal eqâ‚ | Pair-equal eqâ‚‚
            ... | injâ‚ (refl , refl) | injâ‚ (refl , refl) = refl , refl
            ... | injâ‚ (refl , refl) | injâ‚‚ (refl , refl) = refl , refl
            ... | injâ‚‚ (refl , refl) | injâ‚ (refl , refl) = refl , refl
            ... | injâ‚‚ (refl , refl) | injâ‚‚ (refl , refl) = refl , refl

        Pair-ordered : âŸª x , y âŸ« â‰¡ âŸª z , w âŸ« -> (x â‰¡ z) * (y â‰¡ w)
        Pair-ordered {x} {y} {z} {w} eq
            rewrite singleton-pair {x} rewrite singleton-pair {z}
            with Pair-equal eq
        ... | injâ‚ eqâ‚ = Pair-zig x y z w eqâ‚
        ... | injâ‚‚ eqâ‚‚ = Pair-zag x y z w eqâ‚‚

-- Now we can form pairwise unions and intersections.
module Pairwise-Union where
    infixl 15 _âˆª_
    abstract
        _âˆª_ : ğ• -> ğ• -> ğ•
        x âˆª y = â‹ƒ âŸ¨ x , y âŸ©

        private
            Pairwise-Union-> : (x y z : ğ•)
                -> z âˆˆ (x âˆª y) -> (z âˆˆ x) âˆ¨ (z âˆˆ y)
            Pairwise-Union-> x y z (exists .x [ zâˆˆx , Î¹â‚ reflğ• ]) = Î¹â‚ zâˆˆx
            Pairwise-Union-> x y z (exists .y [ zâˆˆy , Î¹â‚‚ reflğ• ]) = Î¹â‚‚ zâˆˆy

            Pairwise-Union<- : (x y z : ğ•)
                -> (z âˆˆ x) âˆ¨ (z âˆˆ y) -> z âˆˆ (x âˆª y)
            Pairwise-Union<- x y z (Î¹â‚ zâˆˆx) = exists x [ zâˆˆx , Î¹â‚ reflğ• ]
            Pairwise-Union<- x y z (Î¹â‚‚ zâˆˆy) = exists y [ zâˆˆy , Î¹â‚‚ reflğ• ]

        Pairwise-Union : (x y z : ğ•)
            -> z âˆˆ (x âˆª y) â‰¡ (z âˆˆ x) âˆ¨ (z âˆˆ y)
        Pairwise-Union x y z = equiv-equal [ Pairwise-Union-> x y z , Pairwise-Union<- x y z ]
open Pairwise-Union public
{-# REWRITE Pairwise-Union #-}

-- We have completely analogous development for intersections.
module Pairwise-Intersection where
    abstract
        infixl 16 _âˆ©_
        _âˆ©_ : ğ• -> ğ• -> ğ•
        x âˆ© y = â‹‚ âŸ¨ x , y âŸ©
        private
            Pairwise-Intersection-> : (x y z : ğ•)
                -> z âˆˆ (x âˆ© y) -> (z âˆˆ x) âˆ§ (z âˆˆ y)
            Pairwise-Intersection-> x y z [ zâˆˆx , zâˆˆy ] =
                [ zâˆˆy x (Î¹â‚ reflğ•) , zâˆˆy y (Î¹â‚‚ reflğ•) ]

            Pairwise-Intersection<- : (x y z : ğ•)
                -> (z âˆˆ x) âˆ§ (z âˆˆ y) -> z âˆˆ (x âˆ© y)
            Pairwise-Intersection<- x y z [ zâˆˆx , zâˆˆy ] =
                [ exists x [ zâˆˆx , Î¹â‚ reflğ• ] ,
                (\ { w (Î¹â‚ reflğ•) -> zâˆˆx ;
                    w (Î¹â‚‚ reflğ•) -> zâˆˆy }) ]

        Pairwise-Intersection : (x y z : ğ•)
            -> z âˆˆ (x âˆ© y) â‰¡ (z âˆˆ x) âˆ§ (z âˆˆ y)
        Pairwise-Intersection x y z = equiv-equal [ Pairwise-Intersection-> x y z , Pairwise-Intersection<- x y z ]
open Pairwise-Intersection public
{-# REWRITE Pairwise-Intersection #-}

-- Regularity
postulate
    Regularity : âˆ€ {a} -> (âˆ€ x -> x âˆˆ a -> âˆƒ[ y âˆˆ ğ• ] (y âˆˆ a âˆ§ y âˆˆ x)) -> a â‰¡ âˆ…

-- A set cannot contain itself.
xâˆ‰x : Â¬ (x âˆˆ x)
xâˆ‰x {x} xâˆˆx = equal-equiv (Extensional-converse âŸ¦xâŸ§â‰¡âˆ… x) reflğ•
    where
        âŸ¦xâŸ§â‰¡âˆ… : âŸ¦ x âŸ§ â‰¡ âˆ…
        âŸ¦xâŸ§â‰¡âˆ… = Regularity \ { _ reflğ• -> exists x [ reflğ• , xâˆˆx ] }

-- Two sets cannot mutually contain each other.
-- This pattern can be continued by induction, but we do not persue this here.
âˆ‰-cycle : (x âˆˆ y) -> (y âˆˆ x) -> âŠ¥ {lzero}
âˆ‰-cycle {x} {y} xâˆˆy yâˆˆx = equal-equiv (Extensional-converse âŸ¨x,yâŸ©â‰¡âˆ… x) (Î¹â‚ reflğ•)
    where
        âŸ¨x,yâŸ©â‰¡âˆ… : âŸ¨ x , y âŸ© â‰¡ âˆ…
        âŸ¨x,yâŸ©â‰¡âˆ… = Regularity \ { w (Î¹â‚ reflğ•) -> exists y [ Î¹â‚‚ reflğ• , yâˆˆx ] ;
                                 w (Î¹â‚‚ reflğ•) -> exists x [ Î¹â‚ reflğ• , xâˆˆy ] }

-- A set cannot contain every set.
ğ•-proper : Â¬ (âˆ€ y -> y âˆˆ x)
ğ•-proper {x} univ = xâˆ‰x {x} (univ x)
-- The consequences of Regularity is profound. So we will not explore them too soon.

-- Infinity
-- Since we have Agda, let's define the set Ï‰ in a really neat way.

-- To be consistent, we use ğŸ˜ as an alias for the empty set.
ğŸ˜ : ğ•
ğŸ˜ = âˆ…

infixl 21 _âº
_âº : ğ• -> ğ•  -- defines the successor
x âº = x âˆª âŸ¦ x âŸ§

-- ğŸ™ is a successor.
ğŸ™â‰¡âˆ…âº : ğŸ™ â‰¡ âˆ… âº
ğŸ™â‰¡âˆ…âº = Extensional zigzag
    where
        zigzag : âˆ€ z -> (z âŠ† âˆ…) â‰¡ âŠ¥ âˆ¨ (z â‰— âˆ…)
        zigzag z rewrite (xâŠ†âˆ… {z}) = equiv-equal [ Î¹â‚‚ , (\ { (Î¹â‚‚ x) -> x }) ]

-- ğŸš is also a successor.
ğŸšâ‰¡ğŸ™âº : ğŸš â‰¡ ğŸ™ âº
ğŸšâ‰¡ğŸ™âº = Extensional \ z -> equiv-equal [ zig , zag ]
    where
        zig : z âˆˆ ğŸš -> (z âŠ† âˆ…) âˆ¨ (z â‰— ğŸ™)
        zig {z} zâˆˆğŸš with ğŸš-boolean {z} zâˆˆğŸš
        ... | injâ‚ refl = Î¹â‚ idP
        ... | injâ‚‚ refl = Î¹â‚‚ reflğ•
        zag : (z âŠ† âˆ…) âˆ¨ (z â‰— ğŸ™) -> z âˆˆ ğŸš
        zag (Î¹â‚ zâŠ†âˆ…) wâˆˆz _ = zâŠ†âˆ… wâˆˆz
        zag (Î¹â‚‚ reflğ•) = idP

-- The successor operation is injective.
injective-âº : âˆ€ x y -> x âº â‰¡ y âº -> x â‰¡ y
injective-âº x y eq = Extensional \ z -> equiv-equal [ zig , zag ]
    where
        ext : (w : ğ•) -> w âˆˆ x âˆ¨ (w â‰— x) â‰¡ w âˆˆ y âˆ¨ (w â‰— y)
        ext = Extensional-converse eq
        zig : z âˆˆ x -> z âˆˆ y
        zig zâˆˆx with equal-equiv (ext _) (Î¹â‚ zâˆˆx) | equal-equiv (ext x) (Î¹â‚‚ reflğ•)
        ... | Î¹â‚ zâˆˆy | _ = zâˆˆy
        ... | Î¹â‚‚ reflğ• | Î¹â‚ xâˆˆy = ex-falso
            (âˆ‰-cycle {y} {x} zâˆˆx xâˆˆy)  -- Since we instantiated a reflğ•, zâˆˆx is actually yâˆˆx.
        ... | Î¹â‚‚ reflğ• | Î¹â‚‚ reflğ• = zâˆˆx
        zag : z âˆˆ y -> z âˆˆ x  -- I didn't bother reusing zig, maybe later..
        zag zâˆˆy with equal-equiv (symm (ext _)) (Î¹â‚ zâˆˆy) | equal-equiv (symm (ext y)) (Î¹â‚‚ reflğ•)
        ... | Î¹â‚ zâˆˆx | _ = zâˆˆx
        ... | Î¹â‚‚ reflğ• | Î¹â‚ yâˆˆx = ex-falso
            (âˆ‰-cycle {x} {y} zâˆˆy yâˆˆx)
        ... | Î¹â‚‚ reflğ• | Î¹â‚‚ reflğ• = zâˆˆy

xâºâ‰¢âˆ… : âˆ€ x -> (x âº â‰¡ âˆ…) -> âŠ¥ {lzero}
xâºâ‰¢âˆ… x eq = equal-equiv (Extensional-converse eq x) (Î¹â‚‚ reflğ•)

-- The ord function embeds Nat into Ï‰.
ord : Nat -> ğ•
ord 0 = ğŸ˜
ord (succ n) = (ord n) âº

injective-ord : âˆ€ n m -> ord n â‰¡ ord m -> n â‰¡ m
injective-ord zero zero eq = refl
injective-ord zero (succ m) eq = magic (xâºâ‰¢âˆ… (ord m) (symm eq))
injective-ord (succ n) zero eq = magic (xâºâ‰¢âˆ… (ord n) eq)
injective-ord (succ n) (succ m) eq
    rewrite injective-ord n m (injective-âº (ord n) (ord m) eq) = refl

-- We now state the axiom of Infinity.
postulate
    Ï‰ : ğ•
    Infinity : âˆ€ n -> ord n âˆˆ Ï‰
    count : âˆ€ x -> .(x âˆˆ Ï‰) -> Nat
    -- ord and count are inverses.
    ord-count : âˆ€ x i -> ord (count x i) â‰¡ x

-- From this, we can prove the other side of the inverse.
count-ord : âˆ€ n i -> count (ord n) i â‰¡ n
count-ord n _ = injective-ord _ _ (ord-count _ _)

{-# REWRITE ord-count count-ord #-}

-- The axiom of choice needs more machinery to state.
-- Therefore, we postpone it.
